new-backend/reg_alloc_translate/reg_alloc_translateScript.sml
@@ -3,12 +3,10 @@ open listTheory arithmeticTheory ml_translatorLib mini_preludeTheory listLib;
 open reg_allocTheory word_procTheory sortingTheory ml_translatorTheory
 open sptreeTheory state_transformerTheory
 open astPP
-open lcsymtacs arithmeticTheory numeralTheory pred_setTheory
+open lcsymtacs numeralTheory pred_setTheory
 open miscLib BasicProvers
 
 val _ = new_theory "reg_alloc_translate";
-
-val _ = translate_into_module "reg_alloc";
 
 val _ = std_preludeLib.std_prelude ();
 
@@ -46,23 +44,9 @@ fun def_of_const tm = let
 val _ = (find_def_for_const := def_of_const);
 
 (* translation *)
-
-val _ = translate lrnext_def
-
-val option_filter_alt = prove(``
-  (option_filter ([]:'a option list) = []) ∧
-  ∀x:'a option xs.
-  (option_filter (x::xs) =
-    case x of NONE => option_filter xs | SOME y => y :: (option_filter xs))``,
-  rw[option_filter_def]>>Cases_on`x`>>fs[])
-
-val def = option_filter_alt |> REWRITE_RULE[] |> curry save_thm"option_filter_alt"
-val _ = translate def
-
-val _ = translate briggs_ok_def
-
 fun fsm ls = fs (ls@[BIND_DEF,UNIT_DEF,IGNORE_BIND_DEF,FOREACH_def]);
 
+(*Use WHILE which is already translated in the prelude*)
 val rpt_do_step_alt = prove(``
   rpt_do_step = \s. ((),WHILE (FST o has_work) (SND o do_step) s)``,
   fs[FUN_EQ_THM,rpt_do_step_def]>>
@@ -102,26 +86,6 @@ val rpt_do_step2_alt = prove(``
   simp[Once whileTheory.WHILE,SimpRHS])
 
 val _ = translate rpt_do_step2_alt
-val _ = translate aux_move_pref_def
-
-val option_CASE_thm = prove(
-  ``option_CASE x f g = case x of NONE => f | SOME y => g y``,
-  CONV_TAC (DEPTH_CONV ETA_CONV) THEN SIMP_TAC std_ss []);
-
-(*Should provide a weakening*)
-val aux_move_pref_side_def = prove(``
-  ∀a b c d e.
-  (d ≠ [] ) ⇒ aux_move_pref_side a b c d e``,
-  rw[fetch"-""aux_move_pref_side_def"])
-
-(*  (d ≠ []) ⇒ aux_move_pref_side a b c d e``,
-  rw[fetch"-""aux_move_pref_side_def",EQ_IMP_THM]) |> update_precondition
-  fs[option_CASE_thm]>>
-  Cases_on`
-  FULL_CASE_TAC>>fs[]>>
-  Cases_on`d`>>fs[]
-  first_match_col_def
-*)
 
 (*Use the clock trick*)
 val rpt_do_step_side_def = prove(``
@@ -139,22 +103,16 @@ val init_ra_state_side_def = prove(``
   fs[MEM_FILTER,MEM_MAP]>>Cases_on`y`>>
   fs[MEM_toAList]) |> update_precondition
 
-val full_coalesce_aux_side_def = prove(``
-  ∀ls G.
-  (∀pxy. MEM pxy ls ⇒let (p:num,x,y) = pxy in
-    x ∈ domain G ∧ y ∈ domain G) ⇒
-  full_coalesce_aux_side G ls``,
-  Induct>>
-  simp[Once (fetch"-""full_coalesce_aux_side_def")]>>
-  rw[]>-
-    cheat (*because we strictly extend the domain*)
-  >>
-  first_x_assum(qspec_then`x4,x2,x1` assume_tac)>>fs[]>>
-  fs[domain_lookup])
+val _ = translate sec_ra_state_def
 
-val _ = translate full_coalesce_def
+val sec_ra_state_side_def = prove(``
+  ∀a b c d. sec_ra_state_side a b c d ⇔ T``,
+  fs[fetch "-" "sec_ra_state_side_def"]>>rw[]>>
+  fs[MEM_FILTER,MEM_MAP,quantHeuristicsTheory.IS_SOME_EQ_NOT_NONE])
+  |>update_precondition
+  
 val irc_alloc_def =  Define`
-  irc_alloc (alg:num) G k moves =
+  irc_alloc G k moves =
   let s = init_ra_state G k moves in
   let s = SND (rpt_do_step s) in
   let coalesced = s.coalesced in
@@ -167,6 +125,23 @@ val irc_alloc_def =  Define`
   let col = spill_coloring G k LN ls col in
     col`
 
+(*Prove that irc alloc is an instance of the actual algorithm*)
+val irc_alloc_reg_alloc_3 = prove(``
+  ∀G k moves.
+  irc_alloc G k moves = reg_alloc 3 G k moves``,
+  fs[irc_alloc_def,reg_alloc_def]>>
+  rw[]>>
+  `pref = pref'` by 
+    (fs[FUN_EQ_THM]>>
+    unabbrev_all_tac>>fs[])>>
+  unabbrev_all_tac>>
+  fs[]>>rfs[]>>
+  rpt VAR_EQ_TAC>>
+  fs[])
+
 val _ = translate irc_alloc_def
+
+val _ = set_trace "pp_avoids_symbol_merges" 0;
+
 
 val _ = export_theory();
